deps/poulet4/lib/P4automata/Benchmarks/Timestamp.v
@@ -17,7 +17,7 @@ Ltac prep_equiv :=
 
 Obligation Tactic := prep_equiv.
 
-Module TimestampRefSingle.
+Module TimestampRefKeepSingle.
   Inductive state :=
   | Start
   | ParseValue1
@@ -209,8 +209,201 @@ Module TimestampRefSingle.
     {| t_states := states |}.
   Solve Obligations with (destruct s; cbv; Lia.lia).
 
-End TimestampRefSingle.
+End TimestampRefKeepSingle.
 
+Module TimestampRefZeroSingle.
+  Inductive state :=
+  | Start
+  | ParseValue1
+  | ParseValue2
+  | ParseValue3
+  | ParseValue4
+  | ParseValue5
+  | ParseValue6.
+
+  Scheme Equality for state.
+
+  Global Instance state_eqdec: EquivDec.EqDec state eq := state_eq_dec.
+  Global Program Instance state_finite: @Finite state _ state_eq_dec :=
+    {| enum := [Start; ParseValue1; ParseValue2; ParseValue3; ParseValue4; ParseValue5; ParseValue6] |}.
+  Next Obligation.
+    repeat constructor;
+      repeat match goal with
+            | H: List.In _ [] |- _ => apply List.in_nil in H; exfalso; exact H
+            | |- ~ List.In _ [] => apply List.in_nil
+            | |- ~ List.In _ (_ :: _) => unfold not; intros
+            | H: List.In _ (_::_) |- _ => inversion H; clear H
+            | _ => discriminate
+            end.
+  Qed.
+  Next Obligation.
+    destruct x; intuition congruence.
+  Qed.
+
+  Inductive header : nat -> Type :=
+  | Typ : header 8
+  | Len : header 8
+  | Value : header 48
+  | Scratch8 : header 8
+  | Scratch16 : header 16
+  | Scratch24 : header 24
+  | Scratch32 : header 32
+  | Scratch40 : header 40.
+
+  Derive Signature for header.
+
+  Definition h16_eq_dec (x y: header 16) : {x = y} + {x <> y} :=
+    match x, y with 
+    | Scratch16, Scratch16 => left eq_refl
+    | _, _ => idProp
+    end.
+
+  Definition h24_eq_dec (x y: header 24) : {x = y} + {x <> y} :=
+    match x, y with 
+    | Scratch24, Scratch24 => left eq_refl
+    | _, _ => idProp
+    end.
+
+  Definition h32_eq_dec (x y: header 32) : {x = y} + {x <> y} :=
+    match x, y with 
+    | Scratch32, Scratch32 => left eq_refl
+    | _, _ => idProp
+    end.
+
+  Definition h40_eq_dec (x y: header 40) : {x = y} + {x <> y} :=
+    match x, y with 
+    | Scratch40, Scratch40 => left eq_refl
+    | _, _ => idProp
+    end.
+
+  Definition h48_eq_dec (x y: header 48) : {x = y} + {x <> y} :=
+    match x, y with 
+    | Value, Value => left eq_refl
+    | _, _ => idProp
+    end.
+
+  Definition h8_eq_dec (x y: header 8) : {x = y} + {x <> y}. 
+  refine (
+    match x with 
+    | Typ => 
+      match y with 
+      | Typ => left eq_refl
+      | Len => right _
+      | Scratch8 => right _
+      end
+    | Len => 
+      match y with 
+      | Typ => right _
+      | Len => left eq_refl
+      | Scratch8 => right _
+      end
+    | Scratch8 => 
+        match y with 
+        | Typ => right _
+        | Len => right _
+        | Scratch8 => left eq_refl
+        end
+    end
+  ); unfold "<>"; intros H; inversion H.
+  Defined.
+
+
+  Definition header_eqdec_ (n: nat) (x: header n) (y: header n) : {x = y} + {x <> y}.
+    solve_header_eqdec_ n x y 
+      ((existT (fun n => forall x y: header n, {x = y} + {x <> y}) _ h8_eq_dec) :: 
+        (existT _ _ h16_eq_dec) :: (existT _ _ h24_eq_dec) :: (existT _ _ h32_eq_dec) :: 
+        (existT _ _ h40_eq_dec) :: (existT _ _ h48_eq_dec) :: nil).
+  Defined. 
+
+  Global Instance header_eqdec: forall n, EquivDec.EqDec (header n) eq := header_eqdec_.
+
+  Global Instance header_eqdec': EquivDec.EqDec (Syntax.H' header) eq.
+  Proof.
+    solve_eqdec'.
+  Defined.
+
+  Global Instance header_finite: forall n, @Finite (header n) _ _.
+  Proof.
+    intros n; solve_indexed_finiteness n [8; 16; 24; 32; 40; 48].
+  Qed.
+
+  Global Program Instance header_finite': @Finite {n & header n} _ header_eqdec' :=
+    {| enum := [ 
+      existT _ _ Len; existT _ _ Typ; existT _ _ Value;  
+      existT _ _ Scratch8; existT _ _ Scratch16; existT _ _ Scratch24;
+      existT _ _ Scratch32; existT _ _ Scratch40
+      
+      ] |}.
+  Next Obligation.
+    solve_header_finite.
+  Qed.
+  Next Obligation.
+  dependent destruction X; subst;
+  repeat (
+    match goal with
+    | |- ?L \/ ?R => (now left; trivial) || right
+    end
+  ).
+  Qed.
+
+  Definition states (s: state) :=
+    match s with
+    | Start =>
+      {| st_op := 
+          extract(Typ) ;;
+          extract(Len) ;
+        st_trans := transition select (| EHdr Len |) {{
+          [| exact #b|0|0|0|0|0|0|0|0 |] ==> accept ;;;
+          [| exact #b|0|0|0|0|0|0|0|1 |] ==> inl ParseValue1 ;;;
+          [| exact #b|0|0|0|0|0|0|1|0 |] ==> inl ParseValue2 ;;;
+          [| exact #b|0|0|0|0|0|0|1|1 |] ==> inl ParseValue3 ;;;
+          [| exact #b|0|0|0|0|0|1|0|0 |] ==> inl ParseValue4 ;;;
+          [| exact #b|0|0|0|0|0|1|0|1 |] ==> inl ParseValue5 ;;;
+          [| exact #b|0|0|0|0|0|1|1|0 |] ==> inl ParseValue6 ;;;
+            reject
+        }}
+      |}
+    | ParseValue1 =>
+      {| st_op := 
+          extract(Scratch8) ;; 
+          Value <- EConcat (n := 8) (EHdr Scratch8) (ELit (Ntuple.n_tuple_repeat 40 false))  ;
+        st_trans := transition accept
+      |}
+    | ParseValue2 =>
+      {| st_op := 
+          extract(Scratch16) ;; 
+          Value <- EConcat (n := 16) (EHdr Scratch16) (ELit (Ntuple.n_tuple_repeat 32 false))  ;
+        st_trans := transition accept
+      |}
+    | ParseValue3 =>
+      {| st_op := 
+          extract(Scratch24) ;; 
+          Value <- EConcat (n := 24) (EHdr Scratch24) (ELit (Ntuple.n_tuple_repeat 24 false))  ;
+        st_trans := transition accept
+      |}
+    | ParseValue4 =>
+      {| st_op := 
+          extract(Scratch32) ;; 
+          Value <- EConcat (n := 32) (EHdr Scratch32) (ELit (Ntuple.n_tuple_repeat 16 false))  ;
+        st_trans := transition accept
+      |}
+    | ParseValue5 =>
+      {| st_op := 
+          extract(Scratch40) ;; 
+          Value <- EConcat (n := 40) (EHdr Scratch40) (ELit (Ntuple.n_tuple_repeat 8 false))  ;
+        st_trans := transition accept
+      |}
+    | ParseValue6 =>
+      {| st_op := extract(Value) ;
+        st_trans := transition accept
+      |}
+    end.
+
+  Program Definition aut: Syntax.t state header :=
+    {| t_states := states |}.
+  Solve Obligations with (destruct s; cbv; Lia.lia).
+
+End TimestampRefZeroSingle.
 
 Module TimestampSpecSingle.
   Inductive state :=
@@ -706,3 +899,492 @@ Module TimestampSpecSmall.
   Solve Obligations with (destruct s; cbv; Lia.lia).
 
 End TimestampSpecSmall.
+
+
+(* parse 3 options of between 0-6 bytes, and if a timestamp option is present, parse it into a timestamp structure *)
+Module TimestampSpec3.
+  Inductive state :=
+  | Parse0
+  | Parse1
+  | Parse2
+
+  | Parse0S
+  | Parse1S
+  | Parse2S
+
+  | Parse01
+  | Parse11
+  | Parse21
+  
+  | Parse02
+  | Parse12
+  | Parse22
+
+  | Parse03
+  | Parse13
+  | Parse23
+
+  | Parse04
+  | Parse14
+  | Parse24
+
+  | Parse05
+  | Parse15
+  | Parse25
+
+  | Parse06
+  | Parse16
+  | Parse26.
+
+  Scheme Equality for state.
+
+  Global Instance state_eqdec: EquivDec.EqDec state eq := state_eq_dec.
+  Global Program Instance state_finite: @Finite state _ state_eq_dec :=
+    {| enum := [  Parse0 ; Parse1; Parse2; 
+    Parse0S ; Parse1S; Parse2S
+    ; Parse01 ; Parse11; Parse21
+      ; Parse02 ; Parse12; Parse22
+    ; Parse03 ; Parse13; Parse23
+    ; Parse04 ; Parse14; Parse24
+    ; Parse05 ; Parse15; Parse25
+    ; Parse06 ; Parse16; Parse26 ]; |}.
+  Next Obligation.
+    repeat constructor;
+      repeat match goal with
+             | H: List.In _ [] |- _ => apply List.in_nil in H; exfalso; exact H
+             | |- ~ List.In _ [] => apply List.in_nil
+             | |- ~ List.In _ (_ :: _) => unfold not; intros
+             | H: List.In _ (_::_) |- _ => inversion H; clear H
+             | _ => discriminate
+             end.
+  Qed.
+  Next Obligation.
+    destruct x; intuition congruence.
+  Qed.
+
+  Inductive header : nat -> Type :=
+  | Scratch8 : header 8
+  | Scratch16 : header 16
+  | Scratch24 : header 24
+  | Scratch32 : header 32
+  | Scratch40 : header 40
+  | T0 : header 8
+  | L0 : header 8
+  | V0 : header 48
+  | T1 : header 8
+  | L1 : header 8
+  | V1 : header 48
+  | T2 : header 8
+  | L2 : header 8
+  | V2 : header 48
+  | Pointer : header 8
+  | Overflow: header 4
+  | Flag: header 4
+  | Timestamp: header 32.
+
+  Derive Signature for header.
+
+  Definition h4_eq_dec (x y: header 4) : {x = y} + {x <> y}.
+  refine (
+    match x, y with
+    | Overflow, Flag => right _
+    | Flag, Overflow => right _
+    | Overflow, Overflow => left eq_refl
+    | Flag, Flag => left eq_refl
+    end
+  ); intros H; inversion H.
+  Defined.
+
+  Definition h8_eq_dec (x y: header 8) : {x = y} + {x <> y}.
+  refine (
+    match x with 
+    | Scratch8 =>
+      match y with
+      | Scratch8  => left eq_refl
+      | T0 => right _
+      | L0 => right _
+      | T1 => right _
+      | L1 => right _
+      | T2 => right _
+      | L2 => right _
+      | Pointer => right _
+      end
+    | T0 =>
+      match y with
+      | Scratch8  => right _
+      | T0 => left eq_refl
+      | L0 => right _
+      | T1 => right _
+      | L1 => right _
+      | T2 => right _
+      | L2 => right _
+      | Pointer => right _
+      end
+      
+    | L0 =>
+      match y with
+      | Scratch8  => right _
+      | T0 => right _
+      | L0 => left eq_refl
+      | T1 => right _
+      | L1 => right _
+      | T2 => right _
+      | L2 => right _
+      | Pointer => right _
+      end
+      
+    | T1 =>
+      match y with
+      | Scratch8  => right _
+      | T0 => right _
+      | L0 => right _
+      | T1 => left eq_refl
+      | L1 => right _
+      | T2 => right _
+      | L2 => right _
+      | Pointer => right _
+      end
+      
+    | L1 =>
+      match y with
+      | Scratch8  => right _
+      | T0 => right _
+      | L0 => right _
+      | T1 => right _
+      | L1 => left eq_refl
+      | T2 => right _
+      | L2 => right _
+      | Pointer => right _
+      end
+    | T2 => 
+      match y with
+      | Scratch8  => right _
+      | T0 => right _
+      | L0 => right _
+      | T1 => right _
+      | L1 => right _
+      | T2 => left eq_refl
+      | L2 => right _
+      | Pointer => right _
+      end
+    | L2 => 
+      match y with
+      | Scratch8  => right _
+      | T0 => right _
+      | L0 => right _
+      | T1 => right _
+      | L1 => right _
+      | T2 => right _
+      | L2 => left eq_refl
+      | Pointer => right _
+      end
+    | Pointer => 
+      match y with
+      | Scratch8  => right _
+      | T0 => right _
+      | L0 => right _
+      | T1 => right _
+      | L1 => right _
+      | T2 => right _
+      | L2 => right _
+      | Pointer => left eq_refl
+      end
+    end
+  ); intros H; inversion H.
+  Defined.
+
+  Definition h16_eq_dec (x y: header 16) : {x = y} + {x <> y} :=
+    match x, y with 
+    | Scratch16, Scratch16 => left eq_refl
+    | _, _ => idProp
+    end.
+  Definition h24_eq_dec (x y: header 24) : {x = y} + {x <> y} :=
+    match x, y with 
+    | Scratch24, Scratch24 => left eq_refl
+    | _, _ => idProp
+    end.
+  Definition h32_eq_dec (x y: header 32) : {x = y} + {x <> y}.
+  refine (
+    match x, y with 
+    | Scratch32, Scratch32 => left eq_refl
+    | Timestamp, Timestamp => left eq_refl
+    | Timestamp, Scratch32 => right _
+    | Scratch32, Timestamp => right _
+    end
+  ); intros H; inversion H.
+  Defined.
+
+  Definition h40_eq_dec (x y: header 40) : {x = y} + {x <> y} :=
+    match x, y with 
+    | Scratch40, Scratch40 => left eq_refl
+    | _, _ => idProp
+    end.
+
+  Definition h48_eq_dec (x y: header 48) : {x = y} + {x <> y}.
+    refine (
+    match x with 
+    | V0 =>
+      match y with
+      | V0 => left eq_refl
+      | V1 => right _
+      | V2 => right _
+      end
+    | V1 =>
+      match y with
+      | V0 => right _
+      | V1 => left eq_refl
+      | V2 => right _
+      end
+    | V2 => 
+      match y with
+      | V0 => right _
+      | V1 => right _
+      | V2 => left eq_refl
+      end
+    end
+  ); intros H; inversion H.
+  Defined.
+
+  Definition header_eqdec_ (n: nat) (x: header n) (y: header n) : {x = y} + {x <> y}.
+    solve_header_eqdec_ n x y 
+      ((existT (fun n => forall x y: header n, {x = y} + {x <> y}) _ h8_eq_dec) :: 
+        (existT _ _ h16_eq_dec) :: (existT _ _ h24_eq_dec) :: (existT _ _ h32_eq_dec) :: 
+        (existT _ _ h40_eq_dec) :: (existT _ _ h48_eq_dec) :: (existT _ _ h4_eq_dec) :: nil).
+  Defined. 
+
+  Global Instance header_eqdec: forall n, EquivDec.EqDec (header n) eq := header_eqdec_.
+
+  Global Instance header_eqdec': EquivDec.EqDec (Syntax.H' header) eq.
+  Proof.
+    solve_eqdec'.
+  Defined.
+
+  Global Instance header_finite: forall n, @Finite (header n) _ _.
+  Proof.
+    intros n; solve_indexed_finiteness n [4; 8; 16; 24; 32; 40; 48].
+  Qed.
+
+  Global Program Instance header_finite': @Finite {n & header n} _ header_eqdec' :=
+    {| enum :=   [existT _ _ Scratch8 ;
+    existT _ _ Scratch16 ;
+    existT _ _ Scratch24 ;
+    existT _ _ Scratch32 ;
+    existT _ _ Scratch40 ;
+    existT _ _ T0 ;
+    existT _ _ L0 ;
+    existT _ _ V0 ;
+    existT _ _ T1 ;
+    existT _ _ L1 ;
+    existT _ _ V1 ;
+    existT _ _ T2 ;
+    existT _ _ L2 ;
+    existT _ _ V2 ;
+    existT _ _ Timestamp ;
+    existT _ _ Pointer ;
+    existT _ _ Overflow ;
+    existT _ _ Flag 
+    ]; |}.
+  Next Obligation.
+    solve_header_finite.
+  Qed.
+  Next Obligation.
+  dependent destruction X; subst;
+  repeat (
+    match goal with
+    | |- ?L \/ ?R => (now left; trivial) || right
+    end
+  ).
+  Qed.
+
+  Definition states (s: state) :=
+    match s with
+    | Parse0 =>
+      {| st_op := 
+          extract(T0) ;;
+          extract(L0) ;
+         st_trans := transition select (| EHdr T0, EHdr L0 |) {{
+           [| exact #b|0|1|0|0|0|1|0|0, exact #b|0|0|0|0|0|1|1|0 |] ==> inl Parse0S;;;
+           [| exact #b|0|0|0|0|0|0|0|0, exact #b|0|0|0|0|0|0|0|0 |] ==> accept ;;;
+           [| exact #b|0|0|0|0|0|0|0|1, exact #b|0|0|0|0|0|0|0|0 |] ==> accept ;;;
+           [| *, exact #b|0|0|0|0|0|0|0|1 |] ==> inl Parse01 ;;;
+           [| *, exact #b|0|0|0|0|0|0|1|0 |] ==> inl Parse02 ;;;
+           [| *, exact #b|0|0|0|0|0|0|1|1 |] ==> inl Parse03 ;;;
+           [| *, exact #b|0|0|0|0|0|1|0|0 |] ==> inl Parse04 ;;;
+           [| *, exact #b|0|0|0|0|0|1|0|1 |] ==> inl Parse05 ;;;
+           [| *, exact #b|0|0|0|0|0|1|1|0 |] ==> inl Parse06 ;;;
+            reject
+         }}
+      |}
+    | Parse01 =>
+      {| st_op := 
+          extract(Scratch8) ;;
+          V0 <- EConcat (m := 40) (EHdr Scratch8) ((EHdr V0)[48--8]) ;
+         st_trans := transition inl Parse1;
+      |}
+    | Parse02 =>
+      {| st_op := 
+          extract(Scratch16) ;;
+          V0 <- EConcat (m := 32) (EHdr Scratch16) ((EHdr V0)[48--16]) ;
+         st_trans := transition inl Parse1;
+      |}
+    | Parse03 =>
+      {| st_op := 
+          extract(Scratch24) ;;
+          V0 <- EConcat (m := 24) (EHdr Scratch24) ((EHdr V0)[48--24]) ;
+         st_trans := transition inl Parse1;
+      |}
+    | Parse04 =>
+      {| st_op := 
+          extract(Scratch32) ;;
+          V0 <- EConcat (m := 16) (EHdr Scratch32) ((EHdr V0)[48--32]) ;
+         st_trans := transition inl Parse1;
+      |}
+    | Parse05 =>
+      {| st_op := 
+          extract(Scratch40) ;;
+          V0 <- EConcat (m := 8) (EHdr Scratch40) ((EHdr V0)[48--40]) ;
+         st_trans := transition inl Parse1;
+      |}
+    | Parse06 =>
+      {| st_op := 
+          extract(V0) ;
+         st_trans := transition inl Parse1;
+      |}
+
+    | Parse0S =>
+      {| st_op := 
+          extract(Pointer) ;;
+          extract(Overflow) ;;
+          extract(Flag) ;;
+          extract(Timestamp) ;
+        st_trans := transition inl Parse1 ;
+      |}
+
+    | Parse1 =>
+      {| st_op := 
+          extract(T1) ;;
+          extract(L1) ;
+         st_trans := transition select (| EHdr T1, EHdr L1 |) {{
+           [| exact #b|0|1|0|0|0|1|0|0, exact #b|0|0|0|0|0|1|1|0 |] ==> inl Parse1S;;;
+           [| exact #b|0|0|0|0|0|0|0|0, exact #b|0|0|0|0|0|0|0|0 |] ==> accept ;;;
+           [| exact #b|0|0|0|0|0|0|0|1, exact #b|0|0|0|0|0|0|0|0 |] ==> accept ;;;
+           [| *, exact #b|0|0|0|0|0|0|0|1 |] ==> inl Parse11 ;;;
+           [| *, exact #b|0|0|0|0|0|0|1|0 |] ==> inl Parse12 ;;;
+           [| *, exact #b|0|0|0|0|0|0|1|1 |] ==> inl Parse13 ;;;
+           [| *, exact #b|0|0|0|0|0|1|0|0 |] ==> inl Parse14 ;;;
+           [| *, exact #b|0|0|0|0|0|1|0|1 |] ==> inl Parse15 ;;;
+           [| *, exact #b|0|0|0|0|0|1|1|0 |] ==> inl Parse16 ;;;
+            reject
+         }}
+      |}
+    | Parse11 =>
+      {| st_op := 
+          extract(Scratch8) ;;
+          V1 <- EConcat (m := 40) (EHdr Scratch8) ((EHdr V1)[48--8]) ;
+         st_trans := transition accept;
+      |}
+    | Parse12 =>
+      {| st_op := 
+          extract(Scratch16) ;;
+          V1 <- EConcat (m := 32) (EHdr Scratch16) ((EHdr V1)[48--16]) ;
+         st_trans := transition accept;
+      |}
+    | Parse13 =>
+      {| st_op := 
+          extract(Scratch24) ;;
+          V1 <- EConcat (m := 24) (EHdr Scratch24) ((EHdr V1)[48--24]) ;
+         st_trans := transition accept;
+      |}
+    | Parse14 =>
+      {| st_op := 
+          extract(Scratch32) ;;
+          V1 <- EConcat (m := 16) (EHdr Scratch32) ((EHdr V1)[48--32]) ;
+         st_trans := transition accept;
+      |}
+    | Parse15 =>
+      {| st_op := 
+          extract(Scratch40) ;;
+          V1 <- EConcat (m := 8) (EHdr Scratch40) ((EHdr V1)[48--40]) ;
+         st_trans := transition accept;
+      |}
+    | Parse16 =>
+      {| st_op := 
+          extract(V1) ;
+         st_trans := transition inl Parse2;
+      |}
+    | Parse1S =>
+      {| st_op := 
+          extract(Pointer) ;;
+          extract(Overflow) ;;
+          extract(Flag) ;;
+          extract(Timestamp) ;
+        st_trans := transition inl Parse2 ;
+      |}
+
+    | Parse2 =>
+      {| st_op := 
+          extract(T2) ;;
+          extract(L2) ;
+         st_trans := transition select (| EHdr T2, EHdr L2 |) {{
+           [| exact #b|0|1|0|0|0|1|0|0, exact #b|0|0|0|0|0|1|1|0 |] ==> inl Parse2S;;;
+           [| exact #b|0|0|0|0|0|0|0|0, exact #b|0|0|0|0|0|0|0|0 |] ==> accept ;;;
+           [| exact #b|0|0|0|0|0|0|0|1, exact #b|0|0|0|0|0|0|0|0 |] ==> accept ;;;
+           [| *, exact #b|0|0|0|0|0|0|0|1 |] ==> inl Parse21 ;;;
+           [| *, exact #b|0|0|0|0|0|0|1|0 |] ==> inl Parse22 ;;;
+           [| *, exact #b|0|0|0|0|0|0|1|1 |] ==> inl Parse23 ;;;
+           [| *, exact #b|0|0|0|0|0|1|0|0 |] ==> inl Parse24 ;;;
+           [| *, exact #b|0|0|0|0|0|1|0|1 |] ==> inl Parse25 ;;;
+           [| *, exact #b|0|0|0|0|0|1|1|0 |] ==> inl Parse26 ;;;
+            reject
+         }}
+      |}
+    | Parse21 =>
+      {| st_op := 
+          extract(Scratch8) ;;
+          V1 <- EConcat (m := 40) (EHdr Scratch8) ((EHdr V2)[48--8]) ;
+         st_trans := transition accept;
+      |}
+    | Parse22 =>
+      {| st_op := 
+          extract(Scratch16) ;;
+          V2 <- EConcat (m := 32) (EHdr Scratch16) ((EHdr V2)[48--16]) ;
+         st_trans := transition accept;
+      |}
+    | Parse23 =>
+      {| st_op := 
+          extract(Scratch24) ;;
+          V2 <- EConcat (m := 24) (EHdr Scratch24) ((EHdr V2)[48--24]) ;
+         st_trans := transition accept;
+      |}
+    | Parse24 =>
+      {| st_op := 
+          extract(Scratch32) ;;
+          V2 <- EConcat (m := 16) (EHdr Scratch32) ((EHdr V2)[48--32]) ;
+         st_trans := transition accept;
+      |}
+    | Parse25 =>
+      {| st_op := 
+          extract(Scratch40) ;;
+          V2 <- EConcat (m := 8) (EHdr Scratch40) ((EHdr V2)[48--40]) ;
+         st_trans := transition accept;
+      |}
+    | Parse26 =>
+      {| st_op := 
+          extract(V2) ;
+         st_trans := transition accept;
+      |}
+    | Parse2S =>
+      {| st_op := 
+          extract(Pointer) ;;
+          extract(Overflow) ;;
+          extract(Flag) ;;
+          extract(Timestamp) ;
+        st_trans := transition accept ;
+      |}
+    end.
+
+  Program Definition aut: Syntax.t state header :=
+    {| t_states := states |}.
+  Solve Obligations with (destruct s; cbv; Lia.lia).
+
+End TimestampSpec3.
